Fix snapshot spec

Examples/SnapshotSpec.v
@@ -12,53 +12,39 @@ Variant SnapSig {A} : ESig :=
 Arguments SnapSig : clear implicits.
 
 Variant SnapState {T A} :=
-| SnapDef (vs : set A) (m : Name T -> option A) (c : Name T -> bool).
+| SnapDef (vs : set A) (m : Name T -> option A).
 Arguments SnapState : clear implicits.
 
 Variant SnapStep {T A} : SnapState T A -> ThreadEvent T (SnapSig A) -> SnapState T A -> Prop :=
-| SnapCallPass i v vs m m' c c' :
-    c i = false ->
-    c' i = true ->
-    differ_pointwise c c' i ->
+| SnapCall i v vs m m' :
     m i = None ->
     m' i = Some v ->
     differ_pointwise m m' i ->
     SnapStep
-      (SnapDef vs m c)
+      (SnapDef vs m)
       (i, CallEv (WriteSnap v))
-      (SnapDef (insert v vs) m' c')
-| SnapRetPass i v vs m m' c :
-    c i = true ->
-    m i = Some v ->
-    m' i = None ->
-    differ_pointwise m m' i ->
-    SnapStep
-      (SnapDef vs m c)
-      (i, RetEv (WriteSnap v) (Some vs))
-      (SnapDef vs m' c)
-| SnapCallFail i v vs m m' c :
-    c i = true ->
+      (SnapDef (insert v vs) m')
+| SnapCallFail i v vs m m' :
     m i = None ->
     m' i = Some v ->
     differ_pointwise m m' i ->
     SnapStep
-      (SnapDef vs m c)
+      (SnapDef vs m)
       (i, CallEv (WriteSnap v))
-      (SnapDef vs m' c)
-| SnapRetFail i v vs m m' c :
-    c i = true ->
+      (SnapDef vs m')
+| SnapRetFail i v vs m m' :
     m i = Some v ->
     m' i = None ->
     differ_pointwise m m' i ->
     SnapStep
-      (SnapDef vs m c)
+      (SnapDef vs m)
       (i, RetEv (WriteSnap v) None)
-      (SnapDef vs m' c).
+      (SnapDef vs m').
 
 Program Definition snapSpec {T A} : Spec T (SnapSig A) := {|
   State := SnapState T A;
   Step := SnapStep;
-  Init := SnapDef emp (fun _ => None) (fun _ => false)
+  Init := SnapDef emp (fun _ => None)
 |}.
 
 Next Obligation.
@@ -81,8 +67,8 @@ Proof.
     now rewrite H.
   }
   cut (
-    forall p vs m c,
-      Steps SnapStep (SnapDef vs m c) p s ->
+    forall p vs m,
+      Steps SnapStep (SnapDef vs m) p s ->
       SeqConsistent (f m) p
   ).
   { intros. now apply H in H0. }
@@ -95,33 +81,16 @@ Proof.
       (a':= f m').
     {
       subst f. simpl.
-      now rewrite H2.
+      now rewrite H.
     }
-    {
-      subst f. simpl.
-      now rewrite H3.
-    }
-    { now apply diff. }
-    {
-      eapply IHp.
-      exact H5.
-    }
-  }
-  {
-    eapply SCRet with
-      (a':= f m').
     {
       subst f. simpl.
       now rewrite H0.
     }
-    {
-      subst f. simpl.
-      now rewrite H1.
-    }
     { now apply diff. }
     {
       eapply IHp.
-      exact H3.
+      exact H2.
     }
   }
   {
@@ -129,16 +98,16 @@ Proof.
       (a':= f m').
     {
       subst f. simpl.
-      now rewrite H0.
+      now rewrite H.
     }
     {
       subst f. simpl.
-      now rewrite H1.
+      now rewrite H0.
     }
     { now apply diff. }
     {
       eapply IHp.
-      exact H3.
+      exact H2.
     }
   }
   {
@@ -146,16 +115,16 @@ Proof.
       (a':= f m').
     {
       subst f. simpl.
-      now rewrite H0.
+      now rewrite H.
     }
     {
       subst f. simpl.
-      now rewrite H1.
+      now rewrite H0.
     }
     { now apply diff. }
     {
       eapply IHp.
-      exact H3.
+      exact H2.
     }
   }
 Qed.
